feat: start implementing multi tree thingy

LeanSAT/Encode/Tseitin.lean
@@ -22,11 +22,11 @@ namespace LeanSAT.Encode.Tseitin
 open Model
 
 inductive NegNormForm (L : Type u)
-| and (a b : NegNormForm L)
-| or (a b : NegNormForm L)
+| all (as : Array (NegNormForm L))
+| any (as : Array (NegNormForm L))
 | tr | fls
 | lit (l : L)
-deriving Repr, DecidableEq
+deriving Repr
 
 namespace NegNormForm
 
@@ -34,8 +34,10 @@ variable [LitVar L ν]
 
 def toPropFun (r : NegNormForm L) : PropFun ν :=
   match r with
-  | .and a b => a.toPropFun ⊓ b.toPropFun
-  | .or a b  => a.toPropFun ⊔ b.toPropFun
+  | .all as => PropFun.all (as.attach.map (fun ⟨x,_h⟩ =>
+      toPropFun x)).toList
+  | .any as => PropFun.any (as.attach.map (fun ⟨x,_h⟩ =>
+      toPropFun x)).toList
   | .lit l => LitVar.toPropFun l
   | .tr => ⊤
   | .fls => ⊥
@@ -56,61 +58,144 @@ def ofPropForm (neg : Bool) : PropForm ν → NegNormForm L
 | .neg f => ofPropForm (!neg) f
 | .conj a b =>
   if neg then
-    .or (ofPropForm neg a) (ofPropForm neg b)
+    .any #[ofPropForm neg a, ofPropForm neg b]
   else
-    .and (ofPropForm neg a) (ofPropForm neg b)
+    .all #[ofPropForm neg a, ofPropForm neg b]
 | .disj a b =>
   if neg then
-    .and (ofPropForm neg a) (ofPropForm neg b)
+    .all #[ofPropForm neg a, ofPropForm neg b]
   else
-    .or (ofPropForm neg a) (ofPropForm neg b)
+    .any #[ofPropForm neg a, ofPropForm neg b]
 | .impl a b =>
   if neg then
-    .and (ofPropForm false a) (ofPropForm true b)
+    .all #[ofPropForm false a, ofPropForm true b]
   else
-    .or (ofPropForm true a) (ofPropForm false b)
+    .any #[ofPropForm true a, ofPropForm false b]
 | .biImpl a b =>
   if neg then
-    .or
-      (.and (ofPropForm false a) (ofPropForm true b))
-      (.and (ofPropForm false b) (ofPropForm true a))
+    .any #[
+      .all #[ofPropForm false a, ofPropForm true b]
+    , .all #[ofPropForm false b, ofPropForm true a]
+    ]
   else
-    .and
-      (.or (ofPropForm true a) (ofPropForm false b))
-      (.or (ofPropForm true b) (ofPropForm false a))
+    .all #[
+      .any #[ofPropForm true a, ofPropForm false b]
+    , .any #[ofPropForm true b, ofPropForm false a]
+    ]
 
 theorem toPropFun_ofPropForm [LawfulLitVar L ν] (f : PropForm ν)
   : toPropFun (L := L) (ofPropForm neg f) =
       if neg then ⟦.neg f⟧ else ⟦f⟧ := by
-  induction f generalizing neg <;>
+  induction f generalizing neg
+  case tr | fls | var | neg | conj | disj | impl | biImpl =>
     -- we ♥ aesop
-    aesop (add norm 1 simp ofPropForm)
-          (add norm 1 simp toPropFun)
-          (add norm 1 simp himp_eq)
-          (add norm 1 simp PropFun.biImpl_eq_impls)
+    aesop (add norm 1 simp [ofPropForm,toPropFun,himp_eq,PropFun.biImpl_eq_impls,Array.attach])
+
+mutual
+def conjuncts : NegNormForm L → Array (NegNormForm L)
+| tr => #[]
+| fls => #[fls]
+| lit l => #[.lit l]
+| all as => as.attach.concatMap (fun ⟨a,_h⟩ => conjuncts a)
+| any as => #[.any <| as.attach.concatMap (fun ⟨a,_h⟩ => disjuncts a)]
+
+def disjuncts : NegNormForm L → Array (NegNormForm L)
+| tr => #[tr]
+| fls => #[]
+| lit l => #[.lit l]
+| any as => as.attach.concatMap (fun ⟨a,_h⟩ => disjuncts a)
+| all as => #[.all <| as.attach.concatMap (fun ⟨a,_h⟩ => conjuncts a)]
+end
+
+set_option maxHeartbeats 500000 in
+set_option pp.proofs.withType false in
+mutual
+def toPropFun_all_conjuncts : (f : NegNormForm L) → toPropFun (.all (conjuncts f)) = toPropFun f
+| tr    => by simp [conjuncts, toPropFun, Array.attach, PropFun.all]
+| fls   => by simp [conjuncts, toPropFun, Array.attach, PropFun.all]
+| lit l => by simp [conjuncts, toPropFun, Array.attach, PropFun.all]
+| all as => by
+  stop
+  have : ∀ a ∈ as, _ := fun a h =>
+    toPropFun_all_conjuncts a
+  ext τ
+  simp_rw [PropFun.ext_iff, imp_forall_iff] at this
+  rw [forall_comm] at this
+  specialize this τ
+  simp (config := {contextual := true})
+    [ toPropFun, Array.attach, @eq_comm _ (toPropFun _)
+    , ← this]
+  clear this
+  simp [conjuncts, Array.data_concatMap, Array.attach, Array.mem_def]
+  constructor
+  · rintro h _ x1 hx1 - rfl - x2 hx2 - -
+    apply h _ _ _ hx1 hx2 _ hx1 hx2 rfl
+  · rintro h _ x2 x1 hx1 hx2 - - - -
+    apply h _ _ hx1 hx1 rfl _ _ hx2 hx2 rfl
+| any as => by
+  stop
+  have : ∀ a ∈ as, _ := fun a h =>
+    toPropFun_any_disjuncts a
+  ext τ
+  simp [toPropFun, conjuncts, Array.data_concatMap, Array.attach, Array.mem_def]
+  constructor
+  · rintro ⟨b,⟨a,ha,hb⟩,h⟩
+    simp_rw [Array.mem_def] at this; specialize this a ha
+    use a; rw [← this]
+    simp [ha, toPropFun, Array.attach]
+    refine ⟨_,⟨b,?_⟩,h⟩
+    simp [hb, Array.mem_def]
+  · rintro ⟨a,ha,h⟩
+    specialize this a; rw [Array.mem_def] at this; specialize this ha
+    rw [← this] at h
+    simp [toPropFun, Array.attach, Array.mem_def] at h
+    rcases h with ⟨b,hb,h⟩
+    refine ⟨b,⟨a,ha,hb⟩,h⟩
+
+def toPropFun_any_disjuncts : (f : NegNormForm L) → toPropFun (.any (disjuncts f)) = toPropFun f
+| tr    => by simp [disjuncts, toPropFun, Array.attach, PropFun.any]
+| fls   => by simp [disjuncts, toPropFun, Array.attach, PropFun.any]
+| lit l => by simp [disjuncts, toPropFun, Array.attach, PropFun.any]
+| any as => by
+  have : ∀ a ∈ as, _ := fun a h =>
+    toPropFun_any_disjuncts a
+  ext τ
+  simp [toPropFun, Array.attach]
+  constructor
+  · rintro ⟨_,⟨b,hb,-,rfl⟩,h⟩
+    simp [disjuncts, Array.data_concatMap, Array.attach] at hb
+    rcases hb with ⟨a,ha,ha',hb⟩
+    specialize this _ ha'
+    refine ⟨_,⟨_,ha,ha',?_⟩,h⟩
+    sorry
+  · sorry
+  stop
+  simp [toPropFun, Array.attach] at this ⊢
+  simp_rw [PropFun.ext_iff, imp_forall_iff] at this
+  rw [forall_comm] at this
+  specialize this τ
+  simp (config := {contextual := true})
+    [ toPropFun, Array.attach, @eq_comm _ (toPropFun _)
+    , ← this]
+  clear this
+  simp [disjuncts, Array.data_concatMap, Array.attach, Array.mem_def]
+  sorry --aesop
+| all as => by
+  have : ∀ a ∈ as, _ := fun a h =>
+    toPropFun_all_conjuncts a
+  sorry
+end
 
 def cleanup : NegNormForm L → NegNormForm L
 | tr => .tr
 | fls => .fls
 | lit l => .lit l
-| and a b =>
-  let a := cleanup a
-  let b := cleanup b
-  match a, b with
-  | .tr, x
-  | x, .tr => x
-  | .fls, _
-  | _, .fls => .fls
-  | _, _ => .and a b
-| or  a b =>
-  let a := cleanup a
-  let b := cleanup b
-  match a, b with
-  | .tr, _
-  | _, .tr => .tr
-  | .fls, x
-  | x, .fls => x
-  | _, _ => .or a b
+| all as =>
+  let conj := conjuncts (.all as)
+  sorry
+| any as =>
+  let disj := disjuncts (.any as)
+  sorry
 
 @[simp] theorem toPropFun_cleanup [LawfulLitVar L ν] (f : NegNormForm L)
   : toPropFun (L := L) (cleanup f) = toPropFun f := by
